Add general tactics

AttarchProperties.v
@@ -1,7 +1,7 @@
 Require Import Ctl.Paths.
 Require Import Ctl.Definition.
+Require Import Ctl.Basic.
 Require Import Ctl.Properties.
-Require Import Ctl.Tactics.
 
 Require Import BinaryRelations.
 Require Import TransitionSystems.
@@ -9,41 +9,63 @@ Require Import Privilege.
 Require Import AttarchTrans.
 
 Require Import Coq.Program.Equality.
+Require Import Ctl.Tactics.
 Require Import Tactics.General.
 Require Import Tactics.Construct.
 
-Definition useram_key_secure : TProp (attarch_global * attarch_state) := 
-  ⟨fun st =>
+Definition useram_key_secure : tprop (attarch_global * attarch_state) := 
+  fun _ st =>
     val_at (useram_key (fst st)) = Some good_useram_key -> 
-    acc_at (useram_key (fst st)) = useram_key_acc
-  ⟩. 
+    acc_at (useram_key (fst st)) = useram_key_acc. 
+
+Ltac tentails :=
+  match goal with 
+  | |- ?R @?s ⊨ ?P => change_no_check (R @s ⊨ P) with (P R s)
+  end.
+
+Tactic Notation "tentails!" :=
+  repeat match goal with 
+  | |- ?R @?s ⊨ ?P => unfold P
+  end;
+  change_no_check (?R @?s ⊨ ?P) with (P R s);
+  cbn.
 
 Theorem useram_key_never_compromised:
   attarch_trans @initial_state_good ⊨ AG useram_key_secure.
 Proof.
+  tsimpl.
   intros n p s' Hin.
-  construct in_path__rtc in Hin.
+  construct in_path__get_prefix_seq in Hin.
   clear p.
   dependent induction Hin.
-  - discriminate.
-  - invc r; try apply IHHin.
+  - tentails. discriminate.
+  - invc r; try (apply IHHin; reflexivity).
     invc H.
-    + invc H1; try apply IHHin.
-      simpl.
+    + invc H1; try (apply IHHin; reflexivity).
+      tentails!.
       reflexivity.
-    + invc H1; try apply IHHin.
-      invc H0; apply IHHin.
+    (* + invc H1; try (apply IHHin; reflexivity).
+      invc H0; apply IHHin; reflexivity. *)
+    + invc H1; [|inv H0]; apply IHHin; reflexivity.
 Qed.
 
-Definition setup_done : TProp (attarch_global * attarch_state) := 
-  ⟨fun st =>
-    snd st = sel4_run (platam_run, vm_run useram_waiting_request)
-  ⟩. 
+Definition setup_done : tprop (attarch_global * attarch_state) := 
+  fun _ st =>
+    snd st = sel4_run (platam_run, vm_run useram_waiting_request). 
 
 Theorem useram_key_never_compromised_setup:
-  attarch_trans @initial_state_good ⊨ A[useram_key_secure U setup_done].
+  attarch_trans @initial_state_good ⊨ A[useram_key_secure W setup_done].
 Proof using.
-  (* expand_tEntails. *)
-  intros n p.
-  destruct exists p m.
-  invc p.
+  rewrite rew_AW.
+  intros n p y i Hin Hprev.
+  let Hin' := fresh in
+    copy Hin Hin';
+    apply in_path_at__get_prefix in Hin' as [p' Hprefix].
+  destruct exists p' curr_state.
+  dependent induction p'.
+  - apply in_path_at_first_inv in Hin as ->.
+    apply tentails_tdisj_l.
+    tentails.
+    discriminate.
+  -
+Abort.
